scf: proof of loop peeling, merges branch scf-theorem
A healthy amount of squashing/simplifying was applied.

Closes: #28

MLIR/Dialects/ScfSemantics.lean
@@ -23,35 +23,59 @@ inductive ScfE: Type -> Type :=
 
 -- | run a loop, decrementing i from n to -
 -- | ix := lo + (n - i) * step
-def run_loop_bounded_go [Monad m] (n: Nat) (i: Nat) (lo: Int) (step: Int)
+def run_loop_bounded_stepped_go [Monad m] (n: Nat) (i: Nat) (lo: Int) (step: Int)
   (accum: a) (eff: Int -> a -> m a): m a := do
    let ix : Int := lo + (n - i) * step
    let accum <- eff ix accum
    match i with
    | .zero => return accum
-   | .succ i' => run_loop_bounded_go n i' lo step accum eff
+   | .succ i' => run_loop_bounded_stepped_go n i' lo step accum eff
 
--- | TODO: use this to run regions.
-def run_loop_bounded [Monad m] (n: Nat) (lo: Int) (step: Int) (accum: a) (eff: Int -> a -> m a): m a :=
-  run_loop_bounded_go n n lo step accum eff
+-- | TODO: make this model the `yield` as well.
+def run_loop_bounded_stepped [Monad m] (n: Nat) (lo: Int) (step: Int) (accum: a) (eff: Int -> a -> m a): m a :=
+  run_loop_bounded_stepped_go n n lo step accum eff
+
+
+-- | TODO: make this model the `yield` as well.
+def run_loop_bounded
+  (n: Nat)
+  (ix: Nat)
+  (start: BlockResult Δ):
+    Fitree (RegionE Δ +' UBE +' ScfE) (BlockResult Δ) := do
+  match n with
+  | 0 => return start
+  | .succ n' => do
+    let (_: BlockResult Δ) <- Fitree.trigger (RegionE.RunRegion 0 [⟨MLIRType.index, ix⟩])
+    run_loop_bounded n' (ix + 1) (.Ret [])
+
 
 -- | TODO: refactor to (1) an effect, (2) an interpretation
 -- | TODO: use the return type of Scf.For. For now, just do unit.
 def scf_semantics_op: IOp Δ →
       Option (Fitree (RegionE Δ +' UBE +' ScfE) (BlockResult Δ))
+
   | IOp.mk "scf.if" [⟨.i1, b⟩] [] 2 _ _ =>
       some (Fitree.trigger <| RegionE.RunRegion (if b == 1 then 0 else 1) [])
-  | IOp.mk "scf.for" [⟨.i32, lo⟩, ⟨.i32, hi⟩, ⟨.i32, step⟩] [] 1 _ _ => some do
-    let nsteps : Int := ((FinInt.toSint'  hi) - (FinInt.toSint' lo)) / FinInt.toSint' step
-    run_loop_bounded
+
+  | IOp.mk "scf.for" [⟨.index, lo⟩, ⟨.index, hi⟩, ⟨.index, step⟩] [] 1 _ _ => some do
+    let nsteps : Int := (hi - lo) / step
+    run_loop_bounded_stepped
       (a := BlockResult Δ)
       (n := nsteps.toNat)
-      (lo := (FinInt.toSint' lo))
-      (step := (FinInt.toSint' step))
+      (lo := lo)
+      (step := step)
       (accum := default)
       (eff := (fun i _ => Fitree.trigger <| RegionE.RunRegion 0 []))
+
+  | IOp.mk "scf.for'" [⟨.index, lo⟩, ⟨.index, hi⟩] [] 1 _ _ => some do
+      run_loop_bounded (n := hi - lo) (ix := lo) (BlockResult.Ret [])
+
   | IOp.mk "scf.yield" vs [] 0 _ _ =>
     some <| return BlockResult.Ret vs
+
+  | IOp.mk "scf.execute_region" args [] 1 _ _ => .some do
+    Fitree.trigger (RegionE.RunRegion 0 args)
+
   | _ => none
 
 def handleScf: ScfE ~> Fitree Void1 :=
@@ -66,7 +90,7 @@ instance: Semantics scf where
 ### Theorems
 -/
 
-namespace scf_th1
+namespace SCF.IF
 -- Proof that `scf.if` with a fixed condition simplifies to its "then" or
 -- "else" region depending on the value
 
@@ -80,8 +104,8 @@ def INPUT (b: Bool): SSAEnv scf := SSAEnv.One [
 
 -- Pure unfolding-style proof
 theorem equivalent (b: Bool):
-    run (denoteRegion _ (LHS r₁ r₂) []) (INPUT b) =
-    run (denoteRegion _ (if b then r₁ else r₂) []) (INPUT b) := by
+    run ⟦LHS r₁ r₂⟧ (INPUT b) =
+    run ⟦if b then r₁ else r₂⟧ (INPUT b) := by
   simp [LHS, INPUT, denoteRegion, denoteBB, denoteBBStmts, denoteTypedArgs]
   simp [denoteBBStmt, denoteOp, List.zip, List.zipWith, List.mapM]
   simp [Semantics.semantics_op, scf_semantics_op]
@@ -90,4 +114,145 @@ theorem equivalent (b: Bool):
   conv in interpSSA' (Fitree.trigger _) => simp [Fitree.trigger]
   simp [SSAEnvE.handle, cast_eq]
   cases b <;> simp [List.get!]
-end scf_th1
+
+end SCF.IF
+
+
+theorem run_bind {Δ: Dialect α' σ' ε'} [S: Semantics Δ] {T R}
+    t (k: T → Fitree (SSAEnvE Δ +' S.E +' UBE) R) env:
+  run (Fitree.bind t k) env =
+    match run t env with
+    | .error ε => .error ε
+    | .ok (x, env') => run (k x) env' := by
+  simp [run]
+  simp [interpSSA'_bind, Fitree.interp'_bind, interpUB_bind]
+  simp [Fitree.run_bind]
+  cases Fitree.run (interpUB _) <;> simp
+
+theorem run_SSAEnvE_get [Δ: Dialect α σ ε] [S: Semantics Δ]
+    (name: SSAVal) (τ: MLIRType Δ) (v: τ.eval) (env: SSAEnv Δ)
+    (k: τ.eval → Fitree (SSAEnvE Δ +' S.E +' UBE) R)
+    (h: SSAEnv.get name τ env = some v):
+  run (Fitree.Vis (Sum.inl <| SSAEnvE.Get τ name) k) env = run (k v) env := by
+  simp [run, SSAEnvE.handle, h]
+
+
+namespace SCF.FOR_PEELING
+def LHS (r: Region scf): Region scf := [mlir_region|
+{
+  "scf.for'" (%c0, %cn_plus_1) ($(r)) : (index, index) -> ()
+}]
+def RHS  (r: Region scf): Region scf := [mlir_region|
+{
+  "scf.execute_region" (%c0) ($(r)) : (index) -> ()
+  "scf.for'" (%c1, %cn_plus_1) ($(r)) : (index, index) -> ()
+}]
+def INPUT (n: Nat): SSAEnv scf := SSAEnv.One [
+  ⟨"cn", .index, n⟩,
+  ⟨"cn_plus_1", .index, n + 1⟩,
+  ⟨"c0", .index, 0⟩,
+  ⟨"c1", .index, 1⟩]
+
+theorem peel_run_loop_bounded {n ix: Nat} (start: BlockResult Δ):
+  run_loop_bounded (n+1) ix start =
+  Fitree.bind (Fitree.trigger <| RegionE.RunRegion 0 [⟨.index, ix⟩])
+    (fun (_: BlockResult Δ) => run_loop_bounded n (ix+1) (.Ret [])) := rfl
+
+-- The main requirement for this theorem is that `r` satisfies SSA invariants,
+-- ie. values available before it runs are unchanged by its execution. Here we
+-- assume something quite a bit stronger, to simplify the proof of the actual
+-- property, which is that a read can commute with running the region.
+
+theorem CORRECT_r (n:Nat) (r: Region scf) args:
+    (run (denoteRegion scf r args) (INPUT n)) = .ok (.Ret [], INPUT n) := by
+  sorry
+
+theorem CORRECT_r_commute_run_interpRegion_SSAEnvE_get [S: Semantics scf]
+  (CORRECT_r: (run (denoteRegion scf r args) (INPUT n)) = .ok (.Ret [], INPUT n))
+  (name: SSAVal) (τ: MLIRType scf) (v: MLIRType.eval τ)
+  (ENV: SSAEnv.get name τ (INPUT n) = some v)
+  (k: BlockResult scf → τ.eval → Fitree (SSAEnvE scf +' Semantics.E scf +' UBE) R):
+  run (Fitree.bind
+    (interpRegion scf [denoteRegion scf r] _ (Sum.inl <| RegionE.RunRegion 0 args))
+    (fun discr =>
+      Fitree.Vis (Sum.inl <| SSAEnvE.Get τ name) fun v => k discr v)) (INPUT n) =
+  run (Fitree.Vis (Sum.inl <| SSAEnvE.Get τ name) fun v =>
+    (Fitree.bind (interpRegion scf [denoteRegion scf r] _ (Sum.inl <| RegionE.RunRegion 0 args))
+    (fun discr => k discr v))) (INPUT n) := by
+  simp [run_bind, interpRegion, List.get!]
+  simp [CORRECT_r]
+  simp [run_SSAEnvE_get _ _ _ _ _ ENV]
+  simp [run_bind, CORRECT_r]
+
+-- Pretty slow due to simplifying scf_semantics_op which contains a large match
+theorem equivalent (n: Nat) (r: Region scf):
+    (run ⟦LHS r⟧ (INPUT n)) =
+    (run ⟦RHS r⟧ (INPUT n)) := by
+  simp [LHS, RHS]
+  simp [denoteRegion, denoteBB, denoteTypedArgs, denoteBBStmts, denoteBBStmt]
+  simp [denoteOp, Semantics.semantics_op, scf_semantics_op]; simp_itree
+  simp [denoteRegions]
+  rw [run_SSAEnvE_get "c0" .index 0]
+  rw [run_SSAEnvE_get "cn_plus_1" .index (n+1)]
+  rw [run_SSAEnvE_get "c0" .index 0]
+  have h := CORRECT_r n r [⟨.index, 0⟩]
+  rw [CORRECT_r_commute_run_interpRegion_SSAEnvE_get h "c1" .index 1]
+  rw [run_SSAEnvE_get "c1" .index 1]
+  rw [CORRECT_r_commute_run_interpRegion_SSAEnvE_get h "cn_plus_1" .index (n+1)]
+  rw [run_SSAEnvE_get "cn_plus_1" .index (n+1)]
+  simp [(by sorry: n + 1 - 1 = n)]
+  simp [peel_run_loop_bounded, Fitree.interp_bind]
+  all_goals simp [INPUT, cast_eq]
+
+end SCF.FOR_PEELING
+
+
+namespace SCF.FOR_FUSION
+def LHS (r: Region scf): Region scf := [mlir_region|
+{
+  "scf.for'" (%c0, %cn) ($(r)) : (index, index) -> ()
+  "scf.for'" (%cn, %cn_plus_m) ($(r)) : (index, index) -> ()
+}]
+def RHS (r: Region scf): Region scf := [mlir_region|
+{
+  "scf.for'" (%c0, %cn_plus_m) ($(r)) : (index, index) -> ()
+}]
+def INPUT (n m: Nat): SSAEnv scf := SSAEnv.One [
+  ⟨"cn", .index, n⟩,
+  ⟨"cn_plus_m", .index, n + m⟩,
+  ⟨"c0", .index, 0⟩]
+
+/- theorem interp_region_of_run_loop_bounded
+  (r: Region scf) (n: Nat)
+  (rhs: Fitree (SSAEnvE scf +' Semantics.E scf +' UBE) (BlockResult scf)):
+    Fitree.interp (interpRegion scf (denoteRegions scf [r]))
+      (run_loop_bounded n 0 (BlockResult.Ret [])) = rhs := by {
+    induction n;
+    case zero => {
+      simp [run_loop_bounded];
+      sorry
+    }
+    case succ n' => {
+      simp [run_loop_bounded];
+      simp [Fitree.interp];
+      sorry
+    }
+   } -/
+
+theorem equivalent (n m: Nat) (r: Region scf):
+    (run ⟦LHS r⟧ (INPUT n m)) =
+    (run ⟦RHS r⟧ (INPUT n m)) := by
+  simp [LHS, RHS, INPUT]
+  simp [denoteRegion, denoteBB, denoteBBStmts, denoteBBStmt, denoteOp]
+  simp_itree
+  simp [Semantics.semantics_op, scf_semantics_op]
+  rw [run_SSAEnvE_get "c0" .index 0]
+  rw [run_SSAEnvE_get "cn" .index n]
+  rw [run_SSAEnvE_get "c0" .index 0]
+  rw [run_SSAEnvE_get "cn_plus_m" .index (n + m)]
+  -- At this point we need something similar to CORRECT_r_* above.
+  -- simp [run_denoteOp_interp_region]
+  sorry
+  all_goals simp [INPUT, cast_eq]
+
+end SCF.FOR_FUSION
